Migrates to type classes & minor improvements.

lean/src/main.lean
@@ -1,23 +1,29 @@
 -- # Abstract Guard Trees
--- This chapter covers basic guards trees with abstract guards.
+-- This chapter covers basic guard trees with abstract guards.
 
--- Represents the type of all guards.
-variable { Grd : Type _ }
+namespace gdt
 
--- Represents the result type of evaluating a guard tree.
-variable { Leaf  : Type _ }
+class GuardModule :=
+    -- Represents the type of all guards.
+    (Grd : Type)
 
--- Represents an environment type that is used to define a semantic for a guard tree.
-variable { Env : Type _ }
+    -- Represents the result type of evaluating a guard tree.
+    (Leaf : Type)
 
+    -- Represents an environment type that is used to define a semantic for a guard tree.
+    (Env : Type)
+
+    -- Describes a semantic for guards.
+    -- None is returned if the guard fails. Guards can modify the environment.
+    -- This abstraction allows for "let x = expr", "x == 1" or "let (Cons x:xs) = list" guards.
+    (grd_eval : Grd → Env → option Env)
+
+
+variable [GuardModule]
+open GuardModule
 
 
 -- ## Guard Trees
--- Semantics of Guards
--- None is returned if the guard fails. Guards can modify the environment.
--- This abstraction allows for "let x = expr", "x == 1" or "let (Cons x:xs) = list" guards.
-class GuardSemantic :=
-(grd_eval : Grd → Env → option Env)
 
 -- This is exactly as defined in the paper, except that guards are abstract.
 inductive Gdt
@@ -25,8 +31,8 @@ inductive Gdt
 | branch : Gdt → Gdt → Gdt
 | grd : Grd → Gdt → Gdt
 
--- Semantics of Guard Trees
-def gdt_eval [@GuardSemantic Grd Env] : @Gdt Grd Leaf → Env → (option (Env × Leaf))
+-- Semantics of Guard Trees. Uses the semantic of guards.
+def gdt_eval : Gdt → Env → (option (Env × Leaf))
 | (Gdt.leaf leaf) env := some (env, leaf)
 | (Gdt.branch tr1 tr2) env :=
     match gdt_eval tr1 env with
@@ -36,16 +42,16 @@ def gdt_eval [@GuardSemantic Grd Env] : @Gdt Grd Leaf → Env → (option (Env �
     | none := gdt_eval tr2 env
     end
 | (Gdt.grd grd tr) env :=
-    match GuardSemantic.grd_eval grd env with
-    -- If guard matches, proceed
+    match grd_eval grd env with
+    -- If guard matches, proceed.
     | some val := gdt_eval tr env
-    -- otherwise, fail.
+    -- Otherwise, fail.
     | none := none
     end
 
 
-
 -- ## Refinement Types
+
 -- This is defined as in the paper, but abstracted over Grd and without a context.
 -- The context is maintained by Env.
 -- An explicit negation of guards is defined here, so guards don't need be closed under negation.
@@ -57,15 +63,15 @@ inductive Φ
 | or : Φ → Φ → Φ
 | and : Φ → Φ → Φ
 
--- Semantics of Refinement Types
-def Φ_eval [@GuardSemantic Grd Env] : @Φ Grd → Env → option Env
+-- This describes the semantic of Refinement Types.
+def Φ_eval: Φ → Env → option Env
 | Φ.false env := none
 | Φ.true env := some env
-| (Φ.grd grd) env := GuardSemantic.grd_eval grd env
+| (Φ.grd grd) env := grd_eval grd env
 | (Φ.negGrd grd) env :=
-    match GuardSemantic.grd_eval grd env with
+    match grd_eval grd env with
     | some env := none
-    -- If a guard fails, it does not modify the environment.
+    -- If a guard fails, it does not modify the environment!
     | none := some env
     end
 | (Φ.or t1 t2) env :=
@@ -84,36 +90,37 @@ def Φ_eval [@GuardSemantic Grd Env] : @Φ Grd → Env → option Env
 
 -- ## Uncovered Refinement Types
 
-def 𝒰_acc : @Φ Grd → @Gdt Grd Leaf → @Φ Grd
+def 𝒰_acc : Φ → Gdt → Φ
 | acc (Gdt.leaf _) := Φ.false
 | acc (Gdt.branch tr1 tr2) := (𝒰_acc (𝒰_acc acc tr1) tr2)
+
 | acc (Gdt.grd grd tree) :=
         Φ.or
             (Φ.and acc $ Φ.negGrd grd)
             (𝒰_acc (Φ.and acc (Φ.grd grd)) tree)
 
-def 𝒰 : @Gdt Grd Leaf → @Φ Grd := 𝒰_acc Φ.true
+def 𝒰 : Gdt → Φ := 𝒰_acc Φ.true
+
 
 -- ### start: optional
 
 -- Alternative definition without accumulator
-def 𝒰' : @Gdt Grd Leaf → @Φ Grd
+def 𝒰' : Gdt → Φ
 | (Gdt.leaf _) := Φ.false
 | (Gdt.branch tr1 tr2) := Φ.and (𝒰' tr1) (𝒰' tr2)
 | (Gdt.grd grd tree) := Φ.or
             (Φ.negGrd grd)
             (Φ.and (Φ.grd grd) (𝒰' tree))
 
--- maybe this lemma is too strong and we can only claim semantic equivalence.
--- Must be weakened in this case.
--- This lemma is not really necessery anyways.
-lemma 𝒰_𝒰'_equiv : ∀ gdt: @Gdt Grd Leaf, 𝒰 gdt = 𝒰' gdt := sorry
+
+lemma 𝒰_𝒰'_equiv : Φ_eval ∘ 𝒰 = Φ_eval ∘ 𝒰' := sorry
 
 -- ### end: optional
 
 -- Uncovered refinement types capture all values that are not covered.
-theorem 𝒰_eval [@GuardSemantic Grd Env] :
-    ∀ env: Env, ∀ gdt: @Gdt Grd Leaf,
+-- This theorem might be easier to show for 𝒰' rather than 𝒰.
+theorem 𝒰_eval :
+    ∀ env: Env, ∀ gdt: Gdt,
         (gdt_eval gdt env ≠ none) ↔ (Φ_eval (𝒰 gdt) env = none)
     := sorry
 
@@ -122,20 +129,20 @@ theorem 𝒰_eval [@GuardSemantic Grd Env] :
 -- ## Annotate
 
 inductive Ant
-| leaf : (@Φ Grd) → Leaf → Ant
+| leaf : Φ → Leaf → Ant
 | branch : Ant → Ant → Ant
 
-def 𝒜_acc : @Φ Grd → @Gdt Grd Leaf → @Ant Grd Leaf
+def 𝒜_acc : Φ → Gdt → Ant
 | acc (Gdt.leaf leaf) := Ant.leaf acc leaf
 | acc (Gdt.branch tr1 tr2) := Ant.branch (𝒜_acc acc tr1) (𝒜_acc (𝒰 tr1) tr2)
 | acc (Gdt.grd grd tr) := (𝒜_acc (Φ.and acc $ Φ.grd grd) tr)
 
-def 𝒜 : @Gdt Grd Leaf → @Ant Grd Leaf := 𝒜_acc Φ.true
+def 𝒜 : Gdt → Ant := 𝒜_acc Φ.true
 
 
 -- Semantics of Ant
 
-def ant_eval [@GuardSemantic Grd Env] : @Ant Grd Leaf → Env → list (Env × Leaf)
+def ant_eval : Ant → Env → list (Env × Leaf)
 | (Ant.leaf ty leaf) env := match (Φ_eval ty env) with
     | none := []
     | (some env) := [(env, leaf)]
@@ -149,9 +156,11 @@ def option_to_list { α: Type _ } : option α → list α
 -- 𝒜 maintains semantics
 -- This theorem implies that ant_eval returns a list of length at most 1.
 -- This means that the refinement types created by 𝒜 are disjoint.
-theorem 𝒜_eval [@GuardSemantic Grd Env] :
-    ∀ env: Env, ∀ gdt: @Gdt Grd Leaf,
+theorem 𝒜_eval :
+    ∀ env: Env, ∀ gdt: Gdt,
         (option_to_list $ gdt_eval gdt env) = ant_eval (𝒜 gdt) env := sorry
+
+end gdt
 
 
 
@@ -164,16 +173,22 @@ theorem 𝒜_eval [@GuardSemantic Grd Env] :
 
 namespace NGdt
 
-variable { Var : Type _ }
+open gdt
+
+class NGuardModule :=
+-- Represents the type of all guards.
+(Grd Leaf Env Var : Type)
+-- None is returned if the guard fails. Guards can modify the environment.
+-- This abstraction allows for "let x = expr", "x == 1" or "let (Cons x:xs) = list" guards.
+(grd_eval : Grd → Env → option Env)
+(isBottom : Var → Env → option Env)
+
+variable [NGuardModule]
+open NGuardModule
 
 inductive NGrd
 | grd: Grd → NGrd
 | bang: Var → NGrd
-
--- Non-Strict Guard Trees can use the bang guard.
-def NGdt :=(@Gdt (@NGrd Grd Var) Leaf)
-
--- ## Semantics of Non-Strict Guard Trees
 
 -- Non-Strict Guard Trees can diverge early with "bottom", so `Leaf` must be extended.
 inductive NLeaf
@@ -186,21 +201,41 @@ inductive XGrd
 | grd: Grd → XGrd
 | isBottom: Var → XGrd
 
-def ngdt_eval [@GuardSemantic (@XGrd Grd Var) Env] : @NGdt Grd Leaf Var → Env → (option (Env × (@NLeaf Leaf)))
-| (Gdt.leaf leaf) env := some (env, NLeaf.leaf leaf)
-| (Gdt.branch tr1 tr2) env :=
+instance GuardModule : gdt.GuardModule := {
+    Grd := XGrd,
+    Leaf := NLeaf,
+    Env := Env,
+    grd_eval := λ grd, match grd with
+    | XGrd.grd grd := grd_eval grd
+    | XGrd.isBottom var := isBottom var
+    end
+}
+
+-- Non-Strict Guard Trees can use the bang guard.
+
+-- ## Semantics of Non-Strict Guard Trees
+
+inductive NGdt
+| leaf : Leaf → NGdt
+| branch : NGdt → NGdt → NGdt
+| grd : NGrd → NGdt → NGdt
+
+
+def ngdt_eval : NGdt → Env → (option (Env × NLeaf))
+| (NGdt.leaf leaf) env := some (env, NLeaf.leaf leaf)
+| (NGdt.branch tr1 tr2) env :=
     match ngdt_eval tr1 env with
     | none := ngdt_eval tr2 env
     | some val := some val
     end
-| (Gdt.grd (NGrd.grd grd) tr) env :=
-    match GuardSemantic.grd_eval ((@XGrd.grd Grd Var) grd) env with
+| (NGdt.grd (NGrd.grd grd) tr) env :=
+    match grd_eval grd env with
     | none := none
     | some val := ngdt_eval tr env
     end
 -- This is the only new case
-| (Gdt.grd (NGrd.bang var) tr) env :=
-    match GuardSemantic.grd_eval ((@XGrd.isBottom Grd Var) var) env with
+| (NGdt.grd (NGrd.bang var) tr) env :=
+    match isBottom var env with
     -- We diverge and exit early, if `var` evaluates to bottom.
     | some val := some (env, NLeaf.bottom)
     -- Otherwise, we continue.
@@ -215,27 +250,26 @@ def ngdt_eval [@GuardSemantic (@XGrd Grd Var) Env] : @NGdt Grd Leaf Var → Env 
 
 -- This transforms a non-strict guard tree to a guard tree with the `isBottom` guard.
 -- The new guard tree can diverge early.
-def ngdt_to_gdt : (@NGdt Grd Leaf Var) → (@Gdt (@XGrd Grd Var) (@NLeaf Leaf))
-| (Gdt.leaf leaf) := (Gdt.leaf (NLeaf.leaf leaf))
-| (Gdt.branch tr1 tr2) := Gdt.branch (ngdt_to_gdt tr1) (ngdt_to_gdt tr2)
-| (Gdt.grd (NGrd.bang var) tr) := Gdt.branch
+def ngdt_to_gdt : NGdt → Gdt
+| (NGdt.leaf leaf) := (Gdt.leaf (NLeaf.leaf leaf))
+| (NGdt.branch tr1 tr2) := Gdt.branch (ngdt_to_gdt tr1) (ngdt_to_gdt tr2)
+| (NGdt.grd (NGrd.bang var) tr) := Gdt.branch
         -- If `var` is bottom, the we diverge with the bottom leaf.
         (Gdt.grd (XGrd.isBottom var) (Gdt.leaf (NLeaf.bottom)))
         -- Otherwise, we continue.
         (ngdt_to_gdt tr)
-| (Gdt.grd (NGrd.grd grd) tr) := (Gdt.grd (XGrd.grd grd) $ ngdt_to_gdt tr)
+| (NGdt.grd (NGrd.grd grd) tr) := (Gdt.grd (XGrd.grd grd) $ ngdt_to_gdt tr)
 
 
 -- Reduction to Guard Trees maintains semantic.
-lemma ngdt_eval_eq_gdt_eval [gs: @GuardSemantic (@XGrd Grd Var) Env] :
-    ∀ gdt: @NGdt Grd Leaf Var, ∀ env: Env,
-        ngdt_eval gdt env = gdt_eval (ngdt_to_gdt gdt) env := sorry
+lemma ngdt_eval_eq_gdt_eval :
+        ngdt_eval = gdt_eval ∘ ngdt_to_gdt := sorry
 
 
-variable is_empty: @Φ Grd → bool
+variable is_empty: Φ → bool
 
 -- returns (accessible, inaccessible, redundant) leaves, given that `is_empty` is correct.
-def ℛ : @Ant Grd NLeaf → list Leaf × list Leaf × list Leaf
+def ℛ : Ant → list Leaf × list Leaf × list Leaf
 | (Ant.leaf ty (NLeaf.leaf n) ) := if is_empty ty then ([], [], [n]) else ([n], [], [])
 | (Ant.leaf ty NLeaf.bottom ) := ([], [], [])
 | (Ant.branch (Ant.leaf ty NLeaf.bottom ) tr2) := 
@@ -249,8 +283,8 @@ def ℛ : @Ant Grd NLeaf → list Leaf × list Leaf × list Leaf
     end
 
 
-def is_correct [@GuardSemantic Grd Env] : (@Φ Grd → bool) → Prop
-| g := ∀ ty: @Φ Grd, (
+def is_correct : (Φ → bool) → Prop
+| g := ∀ ty: Φ, (
         -- If g sais "ty is empty"
         g ty = false →
         -- then `ty` never evaluates to something.
@@ -258,44 +292,43 @@ def is_correct [@GuardSemantic Grd Env] : (@Φ Grd → bool) → Prop
     )
 
 -- Represents all correct G functions from the paper.
-def Gs [@GuardSemantic Grd Env] := { g : @Φ Grd → bool // (@is_correct Grd Env _) g }
+def Gs := { g : Φ → bool // is_correct g }
 
 
 
 -- Removes a list of leaves from a guard tree.
 -- Returns `none` if the guard tree is empty.
-def remove_leaves [decidable_eq Leaf] : list Leaf → (@Gdt Grd Leaf) → option (@Gdt Grd Leaf)
-| leaves (Gdt.leaf leaf) := if leaf ∈ leaves then none else some (Gdt.leaf leaf)
-| leaves (Gdt.branch tr1 tr2) :=
+def remove_leaves [decidable_eq Leaf] : list Leaf → NGdt → option NGdt
+| leaves (NGdt.leaf leaf) := if leaf ∈ leaves then none else some (NGdt.leaf leaf)
+| leaves (NGdt.branch tr1 tr2) :=
     match (remove_leaves leaves tr1, remove_leaves leaves tr2) with
-    | ((some tr1), (some tr2)) := some (Gdt.branch tr1 tr2)
+    | ((some tr1), (some tr2)) := some (NGdt.branch tr1 tr2)
     | ((some tr1), none) := some tr1
     | (none, (some tr2)) := some tr2
     | (none, none) := none
     end
-| leaves (Gdt.grd grd tr) := 
+| leaves (NGdt.grd grd tr) := 
     match remove_leaves leaves tr with
     | none := none
-    | some tr := Gdt.grd grd tr
+    | some tr := NGdt.grd grd tr
     end
 
 -- Like `ngdt_eval` in the `some` case, but never accepts anything in the `none` case.
 -- Catches the semantic of an empty guard tree.
-def ngdt_eval_option [@GuardSemantic (@XGrd Grd Var) Env] : option (@NGdt Grd Leaf Var) → Env → (option (Env × (@NLeaf Leaf)))
+def ngdt_eval_option : option NGdt → Env → (option (Env × NLeaf))
 | (some gdt) env := ngdt_eval gdt env
 | none env := none
 
 -- Every redundant leaf can be marked as inaccessible instead and
 -- every inaccessible leaf can be marked as accessible instead without invalidating the theorem. This only weakens the analysis.
 
-theorem main [decidable_eq Leaf] [@GuardSemantic (@XGrd Grd Var) Env] : ∀ gdt: @NGdt Grd Leaf Var, ∀ is_empty: (@Gs (@XGrd Grd Var) Env _),
+theorem main [decidable_eq Leaf] : ∀ gdt: NGdt, ∀ is_empty: Gs,
     (
         let ⟨ a, i, r ⟩ := ℛ is_empty.val $ 𝒜 $ ngdt_to_gdt gdt
         in
                 -- leaves that are redundant and neither accessible nor inaccessible can be removed without changing semantics
-                ∀ env: Env,
-                    ngdt_eval_option (remove_leaves ((r.remove_all i).remove_all a) gdt) env
-                    = ngdt_eval gdt env
+                ngdt_eval_option (remove_leaves ((r.remove_all i).remove_all a) gdt)
+                = ngdt_eval gdt
             ∧ 
                 -- reachable leaves are accessible.
                 -- Since R is clearly a partition for disjoint leaves,
